Finish sketch of mkParseTableEntries soundness proof

LL1/Proofs/ParseTableGen/mkParseTableEntries_Correctness.v
@@ -1,6 +1,7 @@
 Require Import List.
 
 Require Import Lib.Grammar.
+Require Import Lib.Tactics.
 
 Require Import LL1.ParseTable.
 Require Import LL1.ParseTableGen.
@@ -8,11 +9,17 @@ Require Import LL1.ParseTableGen.
 Definition pt_entries_correct ps g :=
   forall x la gamma,
     In (x, la, gamma) ps <-> lookahead_for la x gamma g.
-
+(*
 Definition entries_correct_wrt_production g es x gamma :=
   forall la, In (x, la, gamma) es <-> lookahead_for la x gamma g.
+ *)
 
 (* invariant relating a list of entries to a list of productions *)
+Definition entries_correct_wrt_productions es ps g :=
+  forall x la gamma,
+    In (x, la, gamma) es <-> In (x, gamma) ps /\ lookahead_for la x gamma g.
+
+(*
 Inductive entries_correct_wrt_productions (g : grammar) :
   list pt_entry -> list production -> Prop :=
 | EntriesCorrect_nil : 
@@ -22,18 +29,63 @@ Inductive entries_correct_wrt_productions (g : grammar) :
       entries_correct_wrt_productions g back_entries ps
       -> entries_correct_wrt_production g front_entries x gamma
       -> entries_correct_wrt_productions g (front_entries ++ back_entries) ((x, gamma) :: ps).
-    
+ *)
+
 Lemma invariant_iff_pt_entries_correct :
   forall es g,
-    entries_correct_wrt_productions g es (productions g) <-> pt_entries_correct es g.
+    entries_correct_wrt_productions es (productions g) g <-> pt_entries_correct es g.
 Proof.
-Admitted.
+  intros es g.
+  split; [intros Hinv | intros Hspec].
+  - unfold entries_correct_wrt_productions, pt_entries_correct in *.
+    intros x la gamma.
+    split; [intros Hin | intros Hlf].
+    + apply Hinv in Hin.
+      destruct Hin; auto.
+    + apply Hinv; split; auto.
+      destruct Hlf; auto.
+  - unfold pt_entries_correct, entries_correct_wrt_productions in *.
+    intros x la gamma.
+    split; [intros Hin | intros [Hin Hlf]].
+    + split.
+      * apply Hspec in Hin.
+        destruct Hin; auto.
+      * apply Hspec; auto.
+    + apply Hspec; auto.
+Qed.
 
 Lemma mkParseTableEntries'_sound :
   forall g nu fi fo ps es,
     mkParseTableEntries' nu fi fo ps = es
-    -> entries_correct_wrt_productions g es ps.
+    -> entries_correct_wrt_productions es ps g.
 Proof.
+  intros g nu fi fo ps.
+  induction ps as [| p ps]; intros es Hmk.
+  - simpl in *; subst.
+    admit.
+  - simpl in *.
+    unfold entries_correct_wrt_productions.
+    intros x la gamma.
+    split; [intros Hin | intros [Hin Hlf]].
+    + subst.
+      apply in_app_or in Hin.
+      destruct Hin.
+      * admit. (* need a lemma about mkEntriesForProd *)
+      * specialize IHps with
+          (es := mkParseTableEntries' nu fi fo ps).
+        unfold entries_correct_wrt_productions in IHps.
+        apply IHps in H; auto.
+        destruct H as [Hin Hlf].
+        split; auto.
+        right; auto.
+    + subst.
+      apply in_or_app.
+      inv Hin.
+      * admit. (* need lemma about mkEntriesForProd *)
+      * right.
+        specialize (IHps (mkParseTableEntries' nu fi fo ps)).
+        unfold entries_correct_wrt_productions in IHps.
+        apply IHps; auto.
 Admitted.
   
 Lemma mkParseTableEntries_sound :
